WIP: The language and the typesystem are now set. We have to define the interpretation for reference types now.

logrel/F_mu_ref.v
@@ -4,6 +4,11 @@ Require Import algebra.upred_big_op.
 Require Import logrel.Vlist.
 
 Module lang.
+
+  Definition loc := positive.
+
+  Instance loc_dec_eq (l l' : loc) : Decision (l = l') := _.
+    
   Inductive expr :=
   | Var (x : var)
   | Lam (e : {bind 1 of expr})
@@ -25,7 +30,7 @@ Module lang.
   | TLam (e : expr)
   | TApp (e : expr)
   (* Reference Types *)
-  | Loc (l : nat)
+  | Loc (l : loc)
   | Alloc (e : expr)
   | Load (e : expr)
   | Store (e1 : expr) (e2 : expr).
@@ -35,6 +40,13 @@ Module lang.
   Instance Subst_expr : Subst expr. derive. Defined.
   Instance SubstLemmas_expr : SubstLemmas expr. derive. Qed.
 
+
+  Instance expr_dec_eq (e e' : expr) : Decision (e = e').
+  Proof.
+    unfold Decision.
+    decide equality; [apply eq_nat_dec | apply loc_dec_eq].
+  Defined.
+  
   Inductive val :=
   | LamV (e : {bind 1 of expr})
   | TLamV (e : {bind 1 of expr})
@@ -43,7 +55,12 @@ Module lang.
   | InjLV (v : val)
   | InjRV (v : val)
   | FoldV (e : expr)
-  | LocV (l : nat).
+  | LocV (l : loc).
+
+  Instance val_dec_eq (v v' : val) : Decision (v = v').
+  Proof.
+    unfold Decision; decide equality; try apply expr_dec_eq; apply loc_dec_eq.
+  Defined.
 
   Fixpoint of_val (v : val) : expr :=
     match v with
@@ -69,7 +86,7 @@ Module lang.
     | Loc l => Some (LocV l)
     | _ => None
     end.
-
+  
   (** Evaluation contexts *)
   Inductive ectx_item :=
   | AppLCtx (e2 : expr)
@@ -111,7 +128,7 @@ Module lang.
   
   Definition fill (K : ectx) (e : expr) : expr := fold_right fill_item e K.
 
-  Definition state : Type := gmap nat val.
+  Definition state : Type := gmap loc val.
 
   Inductive head_step : expr -> state -> expr -> state -> option expr -> Prop :=
   (* β *)
@@ -267,6 +284,15 @@ other words, [e] also contains the reducible expression *)
     eauto using fill_item_no_val_inj, values_head_stuck, fill_not_val.
   Qed.
 
+  Lemma alloc_fresh e v σ :
+    let l := fresh (dom _ σ) in
+    to_val e = Some v → head_step (Alloc e) σ (Loc l) (<[l:=v]>σ) None.
+  Proof. by intros; apply AllocS, (not_elem_of_dom (D:=gset _)), is_fresh. Qed.
+
+  Lemma val_head_stuck e1 σ1 e2 σ2 ef :
+    head_step e1 σ1 e2 σ2 ef → to_val e1 = None.
+  Proof. destruct 1; naive_solver. Qed.
+
 End lang.
 
 (** Language *)
@@ -299,8 +325,8 @@ Proof. change (LanguageCtx lang (lang.fill [Ki])). by apply _. Qed.
 Import lang.
 
 Section lang_rules.
-  From heap_lang Require Export lifting.
-  From algebra Require Import upred_big_op excl dec_agree.
+  From program_logic Require Export lifting.
+  From algebra Require Import upred_big_op frac dec_agree.
   From program_logic Require Export invariants ghost_ownership.
   From program_logic Require Import ownership auth.
   Import uPred.
@@ -308,270 +334,77 @@ Section lang_rules.
    a finmap as their state. Or maybe even beyond "as their state", i.e. arbitrary
    predicates over finmaps instead of just ownP. *)
 
-  Definition heapR : cmraT := mapR loc (exclR (dec_agreeR val)).
+  Definition heapR : cmraT := mapR loc (fracR (dec_agreeR val)).
 
-  (** The CMRA we need. *)
-  Class heapG Σ := HeapG {
-                       heap_inG :> authG heap_lang Σ heapR;
-                       heap_name : gname
-                     }.
-  (** The Functor we need. *)
-  Definition heapGF : gFunctor := authGF heapR.
+(** The CMRA we need. *)
+Class heapG Σ := HeapG {
+  heap_inG :> authG lang Σ heapR;
+  heap_name : gname
+}.
+(** The Functor we need. *)
+Definition heapGF : gFunctor := authGF heapR.
 
-  Definition to_heap : state → heapR := fmap (λ v, Excl (DecAgree v)).
-  Definition of_heap : heapR → state :=
-    omap (mbind (maybe DecAgree) ∘ maybe Excl).
+Definition to_heap : state → heapR := fmap (λ v, Frac 1 (DecAgree v)).
+Definition of_heap : heapR → state :=
+  omap (mbind (maybe DecAgree ∘ snd) ∘ maybe2 Frac).
 
-  Section definitions.
-    Context `{i : heapG Σ}.
+Section definitions.
+  Context `{i : heapG Σ}.
 
-    Definition heap_mapsto (l : loc) (v: val) : iPropG heap_lang Σ :=
-      auth_own heap_name {[ l := Excl (DecAgree v) ]}.
-    Definition heap_inv (h : heapR) : iPropG heap_lang Σ :=
-      ownP (of_heap h).
-    Definition heap_ctx (N : namespace) : iPropG heap_lang Σ :=
-      auth_ctx heap_name N heap_inv.
+  Definition heap_mapsto (l : loc) (q : Qp) (v: val) : iPropG lang Σ :=
+    auth_own heap_name {[ l := Frac q (DecAgree v) ]}.
+  Definition heap_inv (h : heapR) : iPropG lang Σ :=
+    ownP (of_heap h).
+  Definition heap_ctx (N : namespace) : iPropG lang Σ :=
+    auth_ctx heap_name N heap_inv.
 
-    Global Instance heap_inv_proper : Proper ((≡) ==> (≡)) heap_inv.
-    Proof. solve_proper. Qed.
-    Global Instance heap_ctx_always_stable N : AlwaysStable (heap_ctx N).
-    Proof. apply _. Qed.
-  End definitions.
-  Typeclasses Opaque heap_ctx heap_mapsto.
+  Global Instance heap_inv_proper : Proper ((≡) ==> (≡)) heap_inv.
+  Proof. solve_proper. Qed.
+  Global Instance heap_ctx_always_stable N : AlwaysStable (heap_ctx N).
+  Proof. apply _. Qed.
+End definitions.
+Typeclasses Opaque heap_ctx heap_mapsto.
 
-  Notation "l ↦ v" := (heap_mapsto l v) (at level 20) : uPred_scope.
+Notation "l ↦{ q } v" := (heap_mapsto l q v)
+  (at level 20, q at level 50, format "l  ↦{ q }  v") : uPred_scope.
+Notation "l ↦ v" := (heap_mapsto l 1 v) (at level 20) : uPred_scope.
 
-  Section heap.
-    Context {Σ : gFunctors}.
-    Implicit Types N : namespace.
-    Implicit Types P Q : iPropG heap_lang Σ.
-    Implicit Types Φ : val → iPropG heap_lang Σ.
-    Implicit Types σ : state.
-    Implicit Types h g : heapR.
-
-    (** Conversion to heaps and back *)
-    Global Instance of_heap_proper : Proper ((≡) ==> (=)) of_heap.
-    Proof. solve_proper. Qed.
-    Lemma from_to_heap σ : of_heap (to_heap σ) = σ.
-    Proof.
-      apply map_eq=>l. rewrite lookup_omap lookup_fmap. by case (σ !! l).
-    Qed.
-    Lemma to_heap_valid σ : ✓ to_heap σ.
-    Proof. intros l. rewrite lookup_fmap. by case (σ !! l). Qed.
-    Lemma of_heap_insert l v h :
-      of_heap (<[l:=Excl (DecAgree v)]> h) = <[l:=v]> (of_heap h).
-    Proof. by rewrite /of_heap -(omap_insert _ _ _ (Excl (DecAgree v))). Qed.
-    Lemma of_heap_singleton_op l v h :
-      ✓ ({[l := Excl (DecAgree v)]} ⋅ h) →
-      of_heap ({[l := Excl (DecAgree v)]} ⋅ h) = <[l:=v]> (of_heap h).
-    Proof.
-      intros Hv. apply map_eq=> l'; destruct (decide (l' = l)) as [->|].
-      - move: (Hv l). rewrite /of_heap lookup_insert
-                              lookup_omap (lookup_op _ h) lookup_singleton.
-        case _:(h !! l)=>[[[v'|]||]|] //=.
-      - rewrite /of_heap lookup_insert_ne // !lookup_omap.
-          by rewrite (lookup_op _ h) lookup_singleton_ne // left_id.
-    Qed.
-    Lemma to_heap_insert l v σ :
-      to_heap (<[l:=v]> σ) = <[l:=Excl (DecAgree v)]> (to_heap σ).
-    Proof. by rewrite /to_heap -fmap_insert. Qed.
-    Lemma of_heap_None h l :
-      ✓ h → of_heap h !! l = None → h !! l = None ∨ h !! l ≡ Some (Excl DecAgreeBot)
-                                    ∨ h !! l ≡ Some ExclUnit.
-    Proof.
-      move=> /(_ l). rewrite /of_heap lookup_omap.
-        case: (h !! l)=>[[[v|]||]|] //=; destruct 1; auto.
-    Qed.
-    Lemma heap_store_valid l h v1 v2 :
-      ✓ ({[l := Excl (DecAgree v1)]} ⋅ h) →
-      ✓ ({[l := Excl (DecAgree v2)]} ⋅ h).
-    Proof.
-      intros Hv l'; move: (Hv l'). destruct (decide (l' = l)) as [->|].
-      - rewrite !lookup_op !lookup_singleton.
-        case: (h !! l)=>[x|]; [|done]=> /excl_validN_inv_l=>-> //; auto using nat.
-      - by rewrite !lookup_op !lookup_singleton_ne.
-    Qed.
-    Hint Resolve heap_store_valid.
-
-    (** Allocation *)
-    Lemma heap_alloc N E σ :
-      authG heap_lang Σ heapR → nclose N ⊆ E →
-      ownP σ ⊑ (|={E}=> ∃ _ : heapG Σ, heap_ctx N ∧ Π★{map σ} (λ l v, l ↦ v)).
-    Proof.
-      intros. rewrite -{1}(from_to_heap σ). etrans.
-      { rewrite [ownP _]later_intro.
-        apply (auth_alloc (ownP ∘ of_heap) N E (to_heap σ)); last done.
-        apply to_heap_valid. }
-      apply pvs_mono, exist_elim=> γ.
-      rewrite -(exist_intro (HeapG _ _ γ)) /heap_ctx; apply and_mono_r.
-      rewrite /heap_mapsto /heap_name.
-      induction σ as [|l v σ Hl IH] using map_ind.
-      { rewrite big_sepM_empty; apply True_intro. }
-      rewrite to_heap_insert big_sepM_insert //.
-      rewrite (map_insert_singleton_op (to_heap σ));
-        last rewrite lookup_fmap Hl; auto.
-        (* FIXME: investigate why we have to unfold auth_own here. *)
-        by rewrite auth_own_op IH. 
-    Qed.
-
-    Context `{heapG Σ}.
-
-    (** General properties of mapsto *)
-
-    Lemma heap_mapsto_op l v1 v2 :
-      (l ↦ v1 ★ l ↦ v2)%I ≡ (False)%I.
-    Proof.
-      rewrite -auth_own_op map_op_singleton //.
-      
-      
-      apply (anti_symm (⊑)).
-        rewrite auth_own_valid map_validI (forall_elim l) lookup_singleton.
-        rewrite option_validI excl_validI.
-      unfold cmra_op; cbn; trivial.
-      rewrite auth_own_valid map_validI (forall_elim l) lookup_singleton.
-      rewrite option_validI excl_validI.
-      unfold cmra_op; cbn; trivial.
-      
-      apply excl_validN_inv_l.
-      excl_validI discrete_valid. by apply const_elim_r.
-    Qed.
-
-    Lemma heap_mapsto_op_split l q v :
-      (l ↦{q} v)%I ≡ (l ↦{q/2} v ★ l ↦{q/2} v)%I.
-    Proof. by rewrite heap_mapsto_op_eq Qp_div_2. Qed.
-
-    (** Weakest precondition *)
-    Lemma wp_alloc N E e v P Φ :
-      to_val e = Some v →
-      P ⊑ heap_ctx N → nclose N ⊆ E →
-      P ⊑ (▷ ∀ l, l ↦ v -★ Φ (LocV l)) →
-      P ⊑ #> Alloc e @ E {{ Φ }}.
-    Proof.
-      rewrite /heap_ctx /heap_inv=> ??? HP.
-      trans (|={E}=> auth_own heap_name ∅ ★ P)%I.
-      { by rewrite -pvs_frame_r -(auth_empty _ E) left_id. }
-      apply wp_strip_pvs, (auth_fsa heap_inv (wp_fsa (Alloc e)))
-      with N heap_name ∅; simpl; eauto with I.
-      rewrite -later_intro. apply sep_mono_r,forall_intro=> h; apply wand_intro_l.
-      rewrite -assoc left_id; apply const_elim_sep_l=> ?.
-      rewrite -(wp_alloc_pst _ (of_heap h)) //.
-      apply sep_mono_r; rewrite HP; apply later_mono.
-      apply forall_mono=> l; apply wand_intro_l.
-      rewrite always_and_sep_l -assoc; apply const_elim_sep_l=> ?.
-      rewrite -(exist_intro (op {[ l := Frac 1 (DecAgree v) ]})).
-      repeat erewrite <-exist_intro by apply _; simpl.
-      rewrite -of_heap_insert left_id right_id.
-      rewrite /heap_mapsto. ecancel [_ -★ Φ _]%I.
-      rewrite -(map_insert_singleton_op h); last by apply of_heap_None.
-      rewrite const_equiv; last by apply (map_insert_valid h).
-        by rewrite left_id -later_intro.
-    Qed.
-
-    Lemma wp_load N E l q v P Φ :
-      P ⊑ heap_ctx N → nclose N ⊆ E →
-      P ⊑ (▷ l ↦{q} v ★ ▷ (l ↦{q} v -★ Φ v)) →
-      P ⊑ #> Load (Loc l) @ E {{ Φ }}.
-    Proof.
-      rewrite /heap_ctx /heap_inv=> ?? HPΦ.
-      apply (auth_fsa' heap_inv (wp_fsa _) id)
-      with N heap_name {[ l := Frac q (DecAgree v) ]}; simpl; eauto with I.
-      rewrite HPΦ{HPΦ}; apply sep_mono_r, forall_intro=> h; apply wand_intro_l.
-      rewrite -assoc; apply const_elim_sep_l=> ?.
-      rewrite -(wp_load_pst _ (<[l:=v]>(of_heap h))) ?lookup_insert //.
-      rewrite const_equiv // left_id.
-      rewrite /heap_inv of_heap_singleton_op //.
-      apply sep_mono_r, later_mono, wand_intro_l. by rewrite -later_intro.
-    Qed.
-
-    Lemma wp_store N E l v' e v P Φ :
-      to_val e = Some v →
-      P ⊑ heap_ctx N → nclose N ⊆ E →
-      P ⊑ (▷ l ↦ v' ★ ▷ (l ↦ v -★ Φ (LitV LitUnit))) →
-      P ⊑ #> Store (Loc l) e @ E {{ Φ }}.
-    Proof.
-      rewrite /heap_ctx /heap_inv=> ??? HPΦ.
-      apply (auth_fsa' heap_inv (wp_fsa _) (alter (λ _, Frac 1 (DecAgree v)) l))
-      with N heap_name {[ l := Frac 1 (DecAgree v') ]}; simpl; eauto with I.
-      rewrite HPΦ{HPΦ}; apply sep_mono_r, forall_intro=> h; apply wand_intro_l.
-      rewrite -assoc; apply const_elim_sep_l=> ?.
-      rewrite -(wp_store_pst _ (<[l:=v']>(of_heap h))) ?lookup_insert //.
-      rewrite /heap_inv alter_singleton insert_insert !of_heap_singleton_op; eauto.
-      rewrite const_equiv; last naive_solver.
-      apply sep_mono_r, later_mono, wand_intro_l. by rewrite left_id -later_intro.
-    Qed.
-
-    Lemma wp_cas_fail N E l q v' e1 v1 e2 v2 P Φ :
-      to_val e1 = Some v1 → to_val e2 = Some v2 → v' ≠ v1 →
-      P ⊑ heap_ctx N → nclose N ⊆ E →
-      P ⊑ (▷ l ↦{q} v' ★ ▷ (l ↦{q} v' -★ Φ (LitV (LitBool false)))) →
-      P ⊑ #> CAS (Loc l) e1 e2 @ E {{ Φ }}.
-    Proof.
-      rewrite /heap_ctx /heap_inv=>????? HPΦ.
-      apply (auth_fsa' heap_inv (wp_fsa _) id)
-      with N heap_name {[ l := Frac q (DecAgree v') ]}; simpl; eauto 10 with I.
-      rewrite HPΦ{HPΦ}; apply sep_mono_r, forall_intro=> h; apply wand_intro_l.
-      rewrite -assoc; apply const_elim_sep_l=> ?.
-      rewrite -(wp_cas_fail_pst _ (<[l:=v']>(of_heap h))) ?lookup_insert //.
-      rewrite const_equiv // left_id.
-      rewrite /heap_inv !of_heap_singleton_op //.
-      apply sep_mono_r, later_mono, wand_intro_l. by rewrite -later_intro.
-    Qed.
-
-    Lemma wp_cas_suc N E l e1 v1 e2 v2 P Φ :
-      to_val e1 = Some v1 → to_val e2 = Some v2 →
-      P ⊑ heap_ctx N → nclose N ⊆ E →
-      P ⊑ (▷ l ↦ v1 ★ ▷ (l ↦ v2 -★ Φ (LitV (LitBool true)))) →
-      P ⊑ #> CAS (Loc l) e1 e2 @ E {{ Φ }}.
-    Proof.
-      rewrite /heap_ctx /heap_inv=> ???? HPΦ.
-      apply (auth_fsa' heap_inv (wp_fsa _) (alter (λ _, Frac 1 (DecAgree v2)) l))
-      with N heap_name {[ l := Frac 1 (DecAgree v1) ]}; simpl; eauto 10 with I.
-      rewrite HPΦ{HPΦ}; apply sep_mono_r, forall_intro=> h; apply wand_intro_l.
-      rewrite -assoc; apply const_elim_sep_l=> ?.
-      rewrite -(wp_cas_suc_pst _ (<[l:=v1]>(of_heap h))) //;
-                                                         last by rewrite lookup_insert.
-      rewrite /heap_inv alter_singleton insert_insert !of_heap_singleton_op; eauto.
-      rewrite lookup_insert const_equiv; last naive_solver.
-      apply sep_mono_r, later_mono, wand_intro_l. by rewrite left_id -later_intro.
-    Qed.
-  End heap.
+Section heap.
+  Context {Σ : gFunctors}.
+  Implicit Types N : namespace.
+  Implicit Types P Q : iPropG lang Σ.
+  Implicit Types Φ : val → iPropG lang Σ.
+  Implicit Types σ : state.
+  Implicit Types h g : heapR.
 
 
-
-
-
-  Require Import program_logic.lifting.
-
-  Context {Σ : iFunctor}.
-  Implicit Types P : iProp lang Σ.
-  Implicit Types Q : val → iProp lang Σ.
-
-  Lemma wp_bind {E e} K Q :
-    wp E e (λ v, wp E (fill K (of_val v)) Q) ⊑ wp E (fill K e) Q.
+Lemma wp_bind {E e} K Φ :
+    #> e @ E {{ (λ v, #> (fill K (of_val v)) @ E {{Φ}}) }} ⊑ #> (fill K e) @ E {{Φ}}.
   Proof. apply weakestpre.wp_bind. Qed.
 
-  Lemma wp_bindi {E e} Ki Q :
-    wp E e (λ v, wp E (fill_item Ki (of_val v)) Q) ⊑ wp E (fill_item Ki e) Q.
+  Lemma wp_bindi {E e} Ki Φ :
+    #> e @ E {{ (λ v, #> (fill_item Ki (of_val v)) @ E {{Φ}}) }} ⊑ #> (fill_item Ki e) @ E {{Φ}}.
   Proof. apply weakestpre.wp_bind. Qed.
 
   Ltac inv_step :=
-    repeat match goal with
-           | _ => progress simplify_map_eq/= (* simplify memory stuff *)
-           | H : to_val _ = Some _ |- _ => apply of_to_val in H
-           | H : context [to_val (of_val _)] |- _ => rewrite to_of_val in H
-           | H : prim_step _ _ _ _ _ |- _ => destruct H; subst
-           | H : _ = fill ?K ?e |- _ =>
-             destruct K as [|[]];
-               simpl in H; first [subst e|discriminate H|injection H as H]
-           (* ensure that we make progress for each subgoal *)
-           | H : head_step ?e _ _ _ _, Hv : of_val ?v = fill ?K ?e |- _ =>
-             apply values_head_stuck, (fill_not_val K) in H;
-               by rewrite -Hv to_of_val in H (* maybe use a helper lemma here? *)
-           | H : head_step ?e _ _ _ _ |- _ =>
-             try (is_var e; fail 1); (* inversion yields many goals if e is a variable
+      repeat
+      match goal with
+      | _ => progress simplify_map_eq/= (* simplify memory stuff *)
+      | H : to_val _ = Some _ |- _ => apply of_to_val in H
+      | H : context [to_val (of_val _)] |- _ => rewrite to_of_val in H
+      | H : prim_step _ _ _ _ _ |- _ => destruct H; subst
+      | H : _ = fill ?K ?e |- _ =>
+        destruct K as [|[]];
+          simpl in H; first [subst e|discriminate H|injection H as H]
+      (* ensure that we make progress for each subgoal *)
+      | H : head_step ?e _ _ _ _, Hv : of_val ?v = fill ?K ?e |- _ =>
+        apply val_head_stuck, (fill_not_val K) in H;
+          by rewrite -Hv to_of_val in H (* maybe use a helper lemma here? *)
+      | H : head_step ?e _ _ _ _ |- _ =>
+        try (is_var e; fail 1); (* inversion yields many goals if e is a variable
      and can thus better be avoided. *)
-               inversion H; subst; clear H
-           end.
+          inversion H; subst; clear H
+      end.
 
   Ltac reshape_val e tac :=
     let rec go e :=
@@ -581,6 +414,7 @@ Section lang_rules.
           let v1 := reshape_val e1 in let v2 := reshape_val e2 in constr:(PairV v1 v2)
         | InjL ?e => let v := reshape_val e in constr:(InjLV v)
         | InjR ?e => let v := reshape_val e in constr:(InjRV v)
+        | Loc ?l => constr:(LocV l)
         end in let v := go e in first [tac v | fail 2].
 
   Ltac reshape_expr e tac :=
@@ -596,85 +430,280 @@ Section lang_rules.
         | InjL ?e => go (InjLCtx :: K) e
         | InjR ?e => go (InjRCtx :: K) e
         | Case ?e0 ?e1 ?e2 => go (CaseCtx e1 e2 :: K) e0
+        | Alloc ?e => go (AllocCtx :: K) e
+        | Load ?e => go (LoadCtx :: K) e
+        | Store ?e1 ?e2 => reshape_val e1 ltac:(fun v1 => go (StoreRCtx v1 :: K) e2)
+        | Store ?e1 ?e2 => go (StoreLCtx e2 :: K) e1
         end in go (@nil ectx_item) e.
 
   Ltac do_step tac :=
-    try match goal with |- language.reducible _ _ => eexists _, _, _ end;
-    simpl;
-    match goal with
-    | |- prim_step ?e1 ?σ1 ?e2 ?σ2 ?ef =>
-      reshape_expr e1 ltac:(fun K e1' =>
-                              eapply Ectx_step with K e1' _; [reflexivity|reflexivity|];
-                              econstructor;
-                              rewrite ?to_of_val; tac; fail)
-    | |- head_step ?e1 ?σ1 ?e2 ?σ2 ?ef =>
-      econstructor;
-        rewrite ?to_of_val; tac; fail
-    end.
+  try match goal with |- language.reducible _ _ => eexists _, _, _ end;
+  simpl;
+  match goal with
+  | |- prim_step ?e1 ?σ1 ?e2 ?σ2 ?ef =>
+     reshape_expr e1 ltac:(fun K e1' =>
+       eapply Ectx_step with K e1' _; [reflexivity|reflexivity|];
+       first [apply alloc_fresh|econstructor; try reflexivity];
+       rewrite ?to_of_val; tac)
+  | |- head_step ?e1 ?σ1 ?e2 ?σ2 ?ef =>
+     first [apply alloc_fresh|econstructor];
+     rewrite ?to_of_val; tac
+  end.
 
-  Local Hint Extern 1 => do_step auto.
-  Local Hint Extern 1 => inv_step.
+  Local Hint Extern 0 => do_step ltac:(eauto 2).
+  
+  (** Conversion to heaps and back *)
+  Global Instance of_heap_proper : Proper ((≡) ==> (=)) of_heap.
+  Proof. solve_proper. Qed.
+  Lemma from_to_heap σ : of_heap (to_heap σ) = σ.
+  Proof.
+    apply map_eq=>l. rewrite lookup_omap lookup_fmap. by case (σ !! l).
+  Qed.
+  Lemma to_heap_valid σ : ✓ to_heap σ.
+  Proof. intros l. rewrite lookup_fmap. by case (σ !! l). Qed.
+  Lemma of_heap_insert l v h :
+    of_heap (<[l:=Frac 1 (DecAgree v)]> h) = <[l:=v]> (of_heap h).
+  Proof. by rewrite /of_heap -(omap_insert _ _ _ (Frac 1 (DecAgree v))). Qed.
+  Lemma of_heap_singleton_op l q v h :
+    ✓ ({[l := Frac q (DecAgree v)]} ⋅ h) →
+    of_heap ({[l := Frac q (DecAgree v)]} ⋅ h) = <[l:=v]> (of_heap h).
+  Proof.
+    intros Hv. apply map_eq=> l'; destruct (decide (l' = l)) as [->|].
+    - move: (Hv l). rewrite /of_heap lookup_insert
+        lookup_omap (lookup_op _ h) lookup_singleton.
+      case _:(h !! l)=>[[q' [v'|]|]|] //=; last by move=> [??].
+      move=> [? /dec_agree_op_inv [->]]. by rewrite dec_agree_idemp.
+    - rewrite /of_heap lookup_insert_ne // !lookup_omap.
+      by rewrite (lookup_op _ h) lookup_singleton_ne // left_id.
+  Qed.
+  Lemma to_heap_insert l v σ :
+    to_heap (<[l:=v]> σ) = <[l:=Frac 1 (DecAgree v)]> (to_heap σ).
+  Proof. by rewrite /to_heap -fmap_insert. Qed.
+  Lemma of_heap_None h l :
+    ✓ h → of_heap h !! l = None → h !! l = None ∨ h !! l ≡ Some FracUnit.
+  Proof.
+    move=> /(_ l). rewrite /of_heap lookup_omap.
+    by case: (h !! l)=> [[q [v|]|]|] //=; destruct 1; auto.
+  Qed.
+  Lemma heap_store_valid l h v1 v2 :
+    ✓ ({[l := Frac 1 (DecAgree v1)]} ⋅ h) →
+    ✓ ({[l := Frac 1 (DecAgree v2)]} ⋅ h).
+  Proof.
+    intros Hv l'; move: (Hv l'). destruct (decide (l' = l)) as [->|].
+    - rewrite !lookup_op !lookup_singleton.
+      case: (h !! l)=>[x|]; [|done]=> /frac_valid_inv_l=>-> //.
+    - by rewrite !lookup_op !lookup_singleton_ne.
+  Qed.
+  Hint Resolve heap_store_valid.
+
+  (** Allocation *)
+  Lemma heap_alloc N E σ :
+    authG lang Σ heapR → nclose N ⊆ E →
+    ownP σ ⊑ (|={E}=> ∃ _ : heapG Σ, heap_ctx N ∧ Π★{map σ} (λ l v, l ↦ v)).
+  Proof.
+    intros. rewrite -{1}(from_to_heap σ). etrans.
+    { rewrite [ownP _]later_intro.
+      apply (auth_alloc (ownP ∘ of_heap) N E (to_heap σ)); last done.
+      apply to_heap_valid. }
+    apply pvs_mono, exist_elim=> γ.
+    rewrite -(exist_intro (HeapG _ _ γ)) /heap_ctx; apply and_mono_r.
+    rewrite /heap_mapsto /heap_name.
+    induction σ as [|l v σ Hl IH] using map_ind.
+    { rewrite big_sepM_empty; apply True_intro. }
+    rewrite to_heap_insert big_sepM_insert //.
+    rewrite (map_insert_singleton_op (to_heap σ));
+      last rewrite lookup_fmap Hl; auto.
+    (* FIXME: investigate why we have to unfold auth_own here. *)
+    by rewrite auth_own_op IH. 
+  Qed.
+
+  Context `{HGΣ : heapG Σ}.
+
+  (** General properties of mapsto *)
+  Lemma heap_mapsto_op_eq l q1 q2 v :
+    (l ↦{q1} v ★ l ↦{q2} v)%I ≡ (l ↦{q1+q2} v)%I.
+  Proof. by rewrite -auth_own_op map_op_singleton Frac_op dec_agree_idemp. Qed.
+
+  Lemma heap_mapsto_op l q1 q2 v1 v2 :
+    (l ↦{q1} v1 ★ l ↦{q2} v2)%I ≡ (v1 = v2 ∧ l ↦{q1+q2} v1)%I.
+  Proof.
+    destruct (decide (v1 = v2)) as [->|].
+    { by rewrite heap_mapsto_op_eq const_equiv // left_id. }
+    rewrite -auth_own_op map_op_singleton Frac_op dec_agree_ne //.
+    apply (anti_symm (⊑)); last by apply const_elim_l.
+    rewrite auth_own_valid map_validI (forall_elim l) lookup_singleton.
+    rewrite option_validI frac_validI discrete_valid. by apply const_elim_r.
+  Qed.
+
+  Lemma heap_mapsto_op_split l q v :
+    (l ↦{q} v)%I ≡ (l ↦{q/2} v ★ l ↦{q/2} v)%I.
+  Proof. by rewrite heap_mapsto_op_eq Qp_div_2. Qed.
+
+  (** Base axioms for core primitives of the language: Stateful reductions. *)
+  Lemma wp_alloc_pst E σ e v Φ :
+    to_val e = Some v →
+    (▷ ownP σ ★ ▷ (∀ l, σ !! l = None ∧ ownP (<[l:=v]>σ) -★ Φ (LocV l)))
+      ⊑ #> Alloc e @ E {{ Φ }}.
+  Proof.
+    intros. set (φ v' σ' ef := ∃ l,
+                    ef = @None expr ∧ v' = LocV l ∧ σ' = <[l:=v]>σ ∧ σ !! l = None).
+    rewrite -(wp_lift_atomic_step (Alloc e) φ σ) // /φ;
+    last by intros; inv_step; eexists; split; [|eexists].
+    apply sep_mono, later_mono; first done.
+    apply forall_intro=>e2; apply forall_intro=>σ2; apply forall_intro=>ef.
+    apply wand_intro_l.
+    rewrite always_and_sep_l -assoc -always_and_sep_l.
+    apply const_elim_l=>-[l [-> [-> [-> ?]]]].
+      by rewrite (forall_elim l) right_id const_equiv // left_id wand_elim_r.
+  Qed.
+
+  Lemma wp_load_pst E σ l v Φ :
+    σ !! l = Some v →
+    (▷ ownP σ ★ ▷ (ownP σ -★ Φ v)) ⊑ #> Load (Loc l) @ E {{ Φ }}.
+  Proof.
+    intros. rewrite -(wp_lift_atomic_det_step σ v σ None) ?right_id //; 
+      last by intros; inv_step; eauto using to_of_val.
+  Qed.
+
+  Lemma wp_store_pst E σ l e v v' Φ :
+    to_val e = Some v → σ !! l = Some v' →
+    (▷ ownP σ ★ ▷ (ownP (<[l:=v]>σ) -★ Φ (UnitV)))
+      ⊑ #> Store (Loc l) e @ E {{ Φ }}.
+  Proof.
+    intros. rewrite -(wp_lift_atomic_det_step σ (UnitV) (<[l:=v]>σ) None)
+      ?right_id //;
+    last by intros; inv_step; eauto.
+  Qed.
+
+  (** Weakest precondition *)
+  Lemma wp_alloc N E e v P Φ :
+    to_val e = Some v →
+    P ⊑ heap_ctx N → nclose N ⊆ E →
+    P ⊑ (▷ ∀ l, l ↦ v -★ Φ (LocV l)) →
+    P ⊑ #> Alloc e @ E {{ Φ }}.
+  Proof.
+    rewrite /heap_ctx /heap_inv=> ??? HP.
+    trans (|={E}=> auth_own heap_name ∅ ★ P)%I.
+    { by rewrite -pvs_frame_r -(auth_empty _ E) left_id. }
+    apply wp_strip_pvs, (auth_fsa heap_inv (wp_fsa (Alloc e)))
+      with N heap_name ∅; simpl; eauto with I.
+    rewrite -later_intro. apply sep_mono_r,forall_intro=> h; apply wand_intro_l.
+    rewrite -assoc left_id; apply const_elim_sep_l=> ?.
+    rewrite -(wp_alloc_pst _ (of_heap h)) //.
+    apply sep_mono_r; rewrite HP; apply later_mono.
+    apply forall_mono=> l; apply wand_intro_l.
+    rewrite always_and_sep_l -assoc; apply const_elim_sep_l=> ?.
+    rewrite -(exist_intro (op {[ l := Frac 1 (DecAgree v) ]})).
+    repeat erewrite <-exist_intro by apply _; simpl.
+    rewrite -of_heap_insert left_id right_id.
+    rewrite /heap_mapsto. ecancel [_ -★ Φ _]%I.
+    rewrite -(map_insert_singleton_op h); last by apply of_heap_None.
+    rewrite const_equiv; last by apply (map_insert_valid h).
+    by rewrite left_id -later_intro.
+  Qed.
+
+  Lemma wp_load N E l q v P Φ :
+    P ⊑ heap_ctx N → nclose N ⊆ E →
+    P ⊑ (▷ l ↦{q} v ★ ▷ (l ↦{q} v -★ Φ v)) →
+    P ⊑ #> Load (Loc l) @ E {{ Φ }}.
+  Proof.
+    rewrite /heap_ctx /heap_inv=> ?? HPΦ.
+    apply (auth_fsa' heap_inv (wp_fsa _) id)
+      with N heap_name {[ l := Frac q (DecAgree v) ]}; simpl; eauto with I.
+    rewrite HPΦ{HPΦ}; apply sep_mono_r, forall_intro=> h; apply wand_intro_l.
+    rewrite -assoc; apply const_elim_sep_l=> ?.
+    rewrite -(wp_load_pst _ (<[l:=v]>(of_heap h))) ?lookup_insert //.
+    rewrite const_equiv // left_id.
+    rewrite /heap_inv of_heap_singleton_op //.
+    apply sep_mono_r, later_mono, wand_intro_l. by rewrite -later_intro.
+  Qed.
+
+  Lemma wp_store N E l v' e v P Φ :
+    to_val e = Some v →
+    P ⊑ heap_ctx N → nclose N ⊆ E →
+    P ⊑ (▷ l ↦ v' ★ ▷ (l ↦ v -★ Φ UnitV)) →
+    P ⊑ #> Store (Loc l) e @ E {{ Φ }}.
+  Proof.
+    rewrite /heap_ctx /heap_inv=> ??? HPΦ.
+    apply (auth_fsa' heap_inv (wp_fsa _) (alter (λ _, Frac 1 (DecAgree v)) l))
+      with N heap_name {[ l := Frac 1 (DecAgree v') ]}; simpl; eauto with I.
+    rewrite HPΦ{HPΦ}; apply sep_mono_r, forall_intro=> h; apply wand_intro_l.
+    rewrite -assoc; apply const_elim_sep_l=> ?.
+    rewrite -(wp_store_pst _ (<[l:=v']>(of_heap h))) ?lookup_insert //.
+    rewrite /heap_inv alter_singleton insert_insert !of_heap_singleton_op; eauto.
+    rewrite const_equiv; last naive_solver.
+    apply sep_mono_r, later_mono, wand_intro_l. by rewrite left_id -later_intro.
+  Qed.
 
   (** Helper Lemmas for weakestpre. *)
 
-  Lemma wp_lam E e1 e2 v Q :
-    to_val e2 = Some v → ▷ wp E e1.[e2 /] Q ⊑ wp E (App (Lam e1) e2) Q.
+  Lemma wp_lam E e1 e2 v Φ :
+    to_val e2 = Some v → ▷ #> e1.[e2 /] @ E {{Φ}} ⊑ #> (App (Lam e1) e2) @ E {{Φ}}.
   Proof.
     intros <-%of_to_val.
-    rewrite -(wp_lift_pure_det_step (App _ _) e1.[of_val v /] None) //=; auto.
+    rewrite -(wp_lift_pure_det_step (App _ _) e1.[of_val v /] None) //=.
     - by rewrite right_id.
+    - intros. inv_step; auto.
   Qed.
 
-  Lemma wp_TLam E e Q :
-    ▷ wp E e Q ⊑ wp E (TApp (TLam e)) Q.
+  Lemma wp_TLam E e Φ :
+    ▷ #> e @ E {{Φ}} ⊑ #> (TApp (TLam e)) @ E {{Φ}}.
   Proof.
-    rewrite -(wp_lift_pure_det_step (TApp _) e None) //=; auto.
+    rewrite -(wp_lift_pure_det_step (TApp _) e None) //=.
     - by rewrite right_id.
+    - intros. inv_step; auto.
   Qed.
 
-  Lemma wp_Fold E e Q :
-    ▷ wp E e Q ⊑ wp E (Unfold (Fold e)) Q.
+  Lemma wp_Fold E e Φ :
+    ▷ #> e @ E {{Φ}} ⊑ #> (Unfold (Fold e)) @ E {{Φ}}.
   Proof.
-    rewrite -(wp_lift_pure_det_step (Unfold _) e None) //=; auto.
+    rewrite -(wp_lift_pure_det_step (Unfold _) e None) //=.
     - by rewrite right_id.
+    - intros. inv_step; auto.
   Qed.
   
-  Lemma wp_fst E e1 v1 e2 v2 Q :
+  Lemma wp_fst E e1 v1 e2 v2 Φ :
     to_val e1 = Some v1 → to_val e2 = Some v2 →
-    ▷Q v1 ⊑ wp E (Fst (Pair e1 e2)) Q.
+    ▷ Φ v1 ⊑ #> (Fst (Pair e1 e2)) @ E {{Φ}}.
   Proof.
     intros <-%of_to_val <-%of_to_val.
-    rewrite -(wp_lift_pure_det_step (Fst (Pair _ _)) (of_val v1) None) //=; auto.
+    rewrite -(wp_lift_pure_det_step (Fst (Pair _ _)) (of_val v1) None) //=.
     - rewrite right_id; auto using uPred.later_mono, wp_value'.
+    - intros. inv_step; auto.
   Qed.
 
-  Lemma wp_snd E e1 v1 e2 v2 Q :
+  Lemma wp_snd E e1 v1 e2 v2 Φ :
     to_val e1 = Some v1 → to_val e2 = Some v2 →
-    ▷ Q v2 ⊑ wp E (Snd (Pair e1 e2)) Q.
+    ▷ Φ v2 ⊑ #> (Snd (Pair e1 e2)) @ E {{Φ}}.
   Proof.
     intros <-%of_to_val <-%of_to_val.
-    rewrite -(wp_lift_pure_det_step (Snd (Pair _ _)) (of_val v2) None) //=; auto.
+    rewrite -(wp_lift_pure_det_step (Snd (Pair _ _)) (of_val v2) None) //=.
     - rewrite right_id; auto using uPred.later_mono, wp_value'.
+    - intros. inv_step; auto.
   Qed.
 
-  Lemma wp_case_inl E e0 v0 e1 e2 Q :
+  Lemma wp_case_inl E e0 v0 e1 e2 Φ :
     to_val e0 = Some v0 →
-    ▷ wp E e1.[e0/] Q ⊑ wp E (Case (InjL e0) e1 e2) Q.
+    ▷ #> e1.[e0/] @ E {{Φ}} ⊑ #> (Case (InjL e0) e1 e2) @ E {{Φ}}.
   Proof.
     intros <-%of_to_val.
-    rewrite -(wp_lift_pure_det_step (Case (InjL _) _ _) (e1.[of_val v0/]) None) //=; auto.
+    rewrite -(wp_lift_pure_det_step (Case (InjL _) _ _) (e1.[of_val v0/]) None) //=.
     - rewrite right_id; auto using uPred.later_mono, wp_value'.
+    - intros. inv_step; auto.
   Qed.  
 
-  Lemma wp_case_inr E e0 v0 e1 e2 Q :
+  Lemma wp_case_inr E e0 v0 e1 e2 Φ :
     to_val e0 = Some v0 →
-    ▷ wp E e2.[e0/] Q ⊑ wp E (Case (InjR e0) e1 e2) Q.
+    ▷ #> e2.[e0/] @ E {{Φ}} ⊑ #> (Case (InjR e0) e1 e2) @ E {{Φ}}.
   Proof.
     intros <-%of_to_val.
-    rewrite -(wp_lift_pure_det_step (Case (InjR _) _ _) (e2.[of_val v0/]) None) //=; auto.
+    rewrite -(wp_lift_pure_det_step (Case (InjR _) _ _) (e2.[of_val v0/]) None) //=.
     - rewrite right_id; auto using uPred.later_mono, wp_value'.
+    - intros. inv_step; auto.
   Qed.
-  
+
+End heap.
+
 End lang_rules.
 
 Inductive type :=
@@ -1031,11 +1060,8 @@ Section typed_interp.
   Context {Σ : iFunctor}.
   Implicit Types P Q R : iProp lang Σ.
   Notation "# v" := (of_val v) (at level 20).
-  Notation "⊤" := coPset_top.
 
   Canonical Structure leibniz_val := leibnizC val.
-
-  Canonical Structure leibniz_le n m := leibnizC (n ≤ m).
   
   Class Val_to_IProp_AlwaysStable (f : leibniz_val -n> iProp lang Σ) :=
     val_to_iprop_always_stable : ∀ v : val, AlwaysStable ((cofe_mor_car _ _ f) v).
